\documentclass[twoside]{article}
\usepackage{../../estilo-ejercicios}

%--------------------------------------------------------
\begin{document}

\title{Ejercicios de Ideals, Varieties, and Algorithms (4ª Edición)}
\author{Diego Pedraza López, Javier Aguilar Martín, Rafael González López}
\maketitle

\begin{ejercicio}{1.4.1}
Consider the equations
\begin{align*}
x^2 + y^2 -1 & = 0\\
xy - 1 & = 0
\end{align*}
which describe the intersection of a circle and a hyperbola.
\begin{enumerate}[a.]
\item Use algebra to eliminate $y$ from the above equations.
\item Show how the polynomial found in part (a) lies in $\gene{x^2+y^2-1, xy-1}$.
\end{enumerate}
\end{ejercicio}

\begin{solucion}
\begin{enumerate}[a.]
\item[]
\item Multiplicando la segunda ecuación por $xy+1$ obtenemos $x^2y^2-1=0$, luego $y^2 = 1/x^2$.
Desde aquí eliminamos $y$ de la primer ecuación: $x^2+1/x^2-1=0$, que es equivalente a $x^4-x^2+1=0$.
\item De como hemos obtenido este polinomio, deducimos que: $$x^4-x^2+1 = (x^2)(x^2+y^2-1)-(xy+1)(xy-1) \in \gene{x^2+y^2-1, xy-1}$$.
\end{enumerate}


\end{solucion}

\newpage

\begin{ejercicio}{1.4.2}
Let $I \subseteq k[x_1,\dots,x_n]$ be an ideal, and let $f_1,\dots,f_s \in k[x_1,\dots,x_n]$. Prove that the following statements are equivalent:
\begin{enumerate}[(i)]
\item $f_1,\dots,f_s \in I$
\item $\langle f_1,\dots,f_s\rangle \subset I$
\end{enumerate}
This fact is useful when you want to show that one ideal is contained in another.
\end{ejercicio}

\begin{solucion}
La implicación $(ii)\Rightarrow(i)$ es evidente, pues $f_1,\dots,f_s \in \gene{f_1,\dots, f_s}$.

Véamos la otra implicación.
Sea $f \in \gene{f_1,\dots,f_s}$.
Entonces existen $g_1,\dots,g_n \in k[x_1,\dots,x_n]$ tal que:
\[ f = g_1 f_1 + g_2 f_2 + \dots + g_n f_n \]
Por las propiedades de los ideales: como $f_i \in I$, $g_i f_i \in I$, luego $g_1 f_1 + g_2 f_2 + \dots + g_n f_n \in I$.
\end{solucion}

\newpage

\begin{ejercicio}{1.4.3}
Use the previous exercise to prove the following equalities of ideals in $\Q[x,y]$:
\begin{enumerate}[a.]
\item $\gene{x+y,x-y} = \gene{x,y}$.
\item $\gene{x+xy, y+xy, x^2, y^2} = \gene{x, y}$.
\item $\gene{2x^2+3y^2-11, x^2-y^2-3} = \gene{x^2-4, y^2-1}$.
\end{enumerate}
This illustrates that the same ideal can have many different bases and that different bases may have different numbers of elements.
\end{ejercicio}
\begin{solucion}\mbox{}
\begin{enumerate}[a.]
\item $x+y \in \gene{x,y}$ y $x-y \in \gene{x,y}$, luego $\gene{x+y,x-y} \subseteq \gene{x,y}$.
$x = \frac{1}{2} (x+y) + \frac{1}{2}  (x-y) \in \gene{x+y,x-y}$ e $y = \frac{1}{2} (x+y) - \frac{1}{2} (x-y) \in \gene{x+y, x-y}$, luego $\gene{x,y} \subseteq \gene{x+y,x-y}$.
\item $\gene{x+xy, y+xy, x^2, y^2} \subseteq \gene{x, y}$ es evidente.
\[ x = (1+x)(x + xy) - x(y+xy) - x^2 \in \gene{x+xy, y+xy, x^2, y^2} \]
\[ y = (1+y)(y + xy) - y(x+xy) - y^2 \in \gene{x+xy, y+xy, x^2, y^2} \]
Luego $\gene{x,y} \subseteq \gene{x+xy, y+xy, x^2, y^2}$.
\item 
\[ 2x^2+3y^2 - 11 = 2(x^2-4)+3(y^2-1) \in \gene{x^2-4, y^2-1} \]
\[ x^2-y^2-3 = (x^2-4) - (y^2-1) \in \gene{x^2-4, y^2-1} \]
Luego $\gene{2x^2+3y^2-11, x^2-y^2-3} \subseteq \gene{x^2-4, y^2-1}$.
Podemos usar estas ecuaciones para despejar la otra base:
\[ x^2-4 = \frac{1}{5} (2x^2+3y^2-11) - \frac{3}{5} (x^2-y^2-3) \]
\[ y^2-1 = \frac{1}{5}(2x^2+3y^2-11) - \frac{2}{5}(x^2-y^2-3) \]
Luego $\gene{2x^2+3y^2-11, x^2-y^2-3} \supseteq \gene{x^2-4, y^2-1}$.
\end{enumerate}
\end{solucion}

\newpage

\begin{ejercicio}{1.4.4}
Prove Proposition 4: If $f_1,\dots,f_s$ and $g_1,\dots,g_t$ are bases of the same ideal in $k[x_1,\dots,x_n]$, so that $\langle f_1,\dots,f_s\rangle = \langle g_1,\dots,g_t\rangle$, then we have $\V(f_1,\dots,f_s) = \V(g_1,\dots,g_t)$.
\end{ejercicio}
\begin{solucion}
Evidente cuando recordamos que $\V(f_1,\dots,f_s) = \V(\gene{f_1,\dots,f_s})$. Sin embargo, este hecho se probará más adelante. Probemos una inclusión, pues la otra es análoga. Sea $I$ el ideal generado, claramente $f_i,g_j\in I$. Como los $f_i$ forman una base del ideal, podemos escribir
$$
g_j = a_{1j}f_1+\dotsc a_{sj}f_s
$$
Luego si $x\in \V(f_1,\dotsc,f_s)$ entonces $f_i(x)=0$ $\forall i$, por lo que $g_j(x)=0$ $\forall j$ y por tanto $x\in \V(g_1,\dotsc,g_t)$.
\end{solucion}

\newpage

\begin{ejercicio}{1.4.5}
Show that $\V(x+xy,y+xy,x^2,y^2) = \V(x,y)$.
\end{ejercicio}
\begin{solucion}
Hemos visto en el Ejercicio \ref{ejer:1.4.3} que $\gene{x+xy,y+xy,x^2,y^2} = \gene{x,y}$.
Este hecho unido con el Ejercicio \ref{ejer:1.4.4} demuestra el resultado.
\end{solucion}

\newpage

\begin{ejercicio}{1.4.6}
The word ``basis'' is used in various ways in mathematicas.
In this exercise, we will see that ``a basis of an ideal'', as defined in this section, is quite different from ``a basis of a subspace'', which is studied in linear algebra.
\begin{enumerate}[a.]
\item Firrst, consider the ideal $I = \gene{x} \subseteq k[x]$.
As an ideal, $I$ has a basis consisting of the one element $x$.
But $I$ can be regarded as a subspace of $k[x]$, which is a vector space of $k$.
Prove that any vector space basis of $I$ over $k$ is infinite.
\item In linear algebra, a basis must span and be linearly independent over $k$, whereas for an ideal, a basis is concerned only with spanning -- there is no mention of any sort of independence.
The reason is that once we allow polynomial coefficients, no independence is possible.
To see this, consider the ideal $\gene{x,y} \subseteq k[x,y]$.
Show that zero can be be written as a linear combination of $y$ and $x$ with nonzero polynomial coefficients.
\item More generally, suppose that $f_1,\dots,f_s$ is the basis of an ideal $I \subseteq k[x_1,\dots,x_n]$.
If $s ≥ 2$ and $f_i \neq 0$ for all $i$, then show that for any $i$ and $j$, zero can be rewritten as a linear combination of $f_i$ and $f_j$ with nonzero polynomial coefficients.
\item As a consequence of the lack of independence is that when we write an element $f \in \gene{f_1,\dots,f_s}$ as $f = \sum_{i=1}^s h_i f_i$, the coefficients $h_i$ are not unique.
As an example, consider $f = x^2 + xy + y^2 \in \gene{x,y}$.
Express $f$ as a linear combination of $x$ and $y$ in two different ways.
\item A basis $f_1,\dots,f_s$ of an ideal $I$ is said to be \emph{minimal} if no proper subset of $f_1,\dots,f_s$ is a basis of $I$. For example, $\{x,x^2\}$ is a basis of an ideal, but not a minimal basis since $x$ generates the same ideal.
Unfortunately, an ideal can have minimal bases consisting of different numbers of elements.
To see this, show that $x$ and $x+x^2,x^2$ are minimal bases of the same ideal $k[x]$. Explain how this contrasts with the situation in linear algebra.
\end{enumerate}
\end{ejercicio}
\begin{solucion}
\begin{enumerate}[a.]
\item[]
\item Como espacio vectorial una base de $I$ es $1,x,x^2,\dots$. Por el Teorema de la base para e.v. tenemos que cualquier otra base tiene el mismo cardinal (en este caso infinito).
Es una base infinita, luego $I$ tiene dimensión infinita como espacio vectorial.
\item $xy-yx = 0$.
\item $f_i f_j - f_j f_i = 0$. Aquí usamos que $f_i \neq 0$ para todo $i$.
\item $x^2+xy+y^2 = (x+y)x+yy = xx+(x+y)y$.
\item Claramente $x$ es una base mínima.
Como ni $x+x^2$ ni $x^2$ genera el mismo ideal que $x+x^2,x^2$, este es mínimo.
Es fácil ver además que $\gene{x}=\gene{x+x^2,x^2}$.
Tenemos aquí un ejemplo de que las bases de ideales no tienen necesariamente la misma cantidad de elementos.
Esto lo diferencia con el caso de álgebra lineal.
\end{enumerate}
\end{solucion}

\newpage

\begin{ejercicio}{1.4.7}
Show that $\I(\V(x^n,y^m))=\langle x,y \rangle$, for any positive integers $n$ and $m$.
\end{ejercicio}
\begin{solucion}
Como $x^n$ e $y^m$ se anulan si y sólo si $x=y=0$, tenemos que $\V(x^n,y^m)= \{(0,0)\}$. Ya sabemos que $\I(\{(0,0)\}) = \gene{x,y}$, de donde se tiene el resultado.
\end{solucion}

\newpage

\begin{ejercicio}{1.4.8}
The ideal $\I(V)$ of a variety has a special property not shared by all ideals. Specifically, we define an ideal $I$ to be \emph{radical} if whenever a power $f^m$ of a polynomial $f$ is in $I$, then $f$ itself is in $I$. More succinctly, $I$ is radical when $f \in I$ if and only if $f^m \in I$ for some positive integer $m$.
\begin{enumerate}[a.]
\item Prove that $\I(V)$ is always a radical ideal.
\item Prove that $\gene{x^2,y^2}$ is not a radical ideal.
This implies that $\gene{x^2,y^2} \neq \I(V)$ for any variety $V \subseteq k^2$.
\end{enumerate}
Radicals ideals will play an important role in Chapter 4. In particular, the Nullstellensatz will imply that there is a one-to-one correspondence between varieties in $\C^n$ and radical ideals in $\C[x_1,\dots,x_n]$.
\end{ejercicio}
\begin{solucion}
\begin{enumerate}[a.]
\item[]
\item Sea $f^m \in \I(V)$ con $f \in k[1,\dots,x_n]$ y $m$ entero positivo.
Supongamos que $V$ es no vacío.
Sea $p \in V$, entonces $f^m(p)=0$.
Como el ideal $\gene{0}$ es primo en $k$, tenemos que $f(p)=0$.
Como $p$ era un punto arbitrario, $f$ se anula en todo $V$, luego $f \in \I(V)$.
Esto demuestra que $\I(V)$ es radical.
\item Claramente $x \notin \gene{x^2,y^2}$, pero $x^2 \in \gene{x^2,y^2}$, luego $\gene{x^2,y^2}$ no es ideal radical.
\end{enumerate}
\end{solucion}
\newpage
\begin{ejercicio}{1.4.9}
Let $V = \V(y − x^2, z − x^3)$ be the twisted cubic. In the text, we showed that $\I(V) = \gene{y − x^2, z − x^3}$.
\begin{enumerate}
\item Use the parametrization of the twisted cubic to show that $y^2 − xz \in \I(V)$.
\item Use the argument given in the text to express $y^2 − xz$ as a combination of $y − x^2$ and $z − x^3$.
\end{enumerate}
\end{ejercicio}
\begin{solucion}
\begin{enumerate}
\item[]
\item Sustituyendo $x\to t$, $y\to t^2$ y $z\to t^3$ es claro que $y^2-xz = t^4-tt^3 = 0$, luego se anula en todos los puntos de la curva.
\item $y^2-xz=-x(z-x^3) + (y+x^2)(y-x^2)$. 
\end{enumerate}
\end{solucion}

\newpage
\begin{ejercicio}{1.4.10}
Use the argument given in the discussion of the twisted cubic to show that $\I(\V(x−y)) = \gene{x-y}$. Your argument should be valid for any infinite field k.
\begin{solucion}
Sabemos que $\V(x-y) = \{(t,t)\mid t\in k\}$. Sea $f\func{k[x,y]}{k[t]}$ de manera que $x\to t$, $y\to t$. Es claro que $\ker f = \gene{x-y}$. Como $k[t]$ es dominio de integridad, $\ker f$ es un ideal primo, luego en particular es una ideal radical. Finalmente, por el Teorema de los ceros de Hilbert tenemos que $\I(\V(S))=\sqrt{\gene{S}}$, de donde se deduce el resultado.
\end{solucion}
\end{ejercicio}

\newpage
\begin{ejercicio}{1.4.11}
Let $V ⊆ \R^3$ be the curve parametrized by $(t, t^3, t^4)$.
\begin{enumerate}[a.]
\item Prove that V is an affine variety.
\item Adapt the method used in the case of the twisted cubic to determine $\I(V)$.
\end{enumerate}
\begin{solucion}
\begin{enumerate}[a.]
\item[]
\item Vamos a ver la curva es precisamente $S=\V(x^3-y,x^4-z)$. Obviamente $V\subset S$. Recíprocamente, sea $(x,y,z)\in S$. Escribiendo $x=t$ entonces $y=x^3=t^3$ y $z=t^4$. Por tanto, $V$ es una variedad afín.
\item Con un procedimiento análogo al que se realiza en la página 33 del libro, podemos ver que todo polinomio $f \in \R[x,y,z]$ puede escribirse como
$$
f = h_1(x^3-y)+h_2(x^4-z)+r
$$
donde $r\in \R[x]$. Es claro que $\gene{x^3-y,x^4-z}\subset I(S)$. Recíprocamente, veamos que si $f\in \I(S)$, $r=0$. Como $f\in I(S)$ entonces $f(t,t^3,t^4)=0$, luego
$$
f(t,t^3,t^4)= h_1(t,t^3,t^4)(t^3-t^3)+h_2(t,t^3,t^4)(t^4-t^4)+r(t) = r(t) = 0$$
Como $r(t)=0$ $\forall t \in \R$ entonces $r=0$. Lo que prueba la igualdad.
\end{enumerate}
\end{solucion}
\end{ejercicio}

\newpage
\begin{ejercicio}{1.4.12}
Let $V ⊆ \R^3$ be the curve parametrized by $(t^2, t^3, t^4)$.
\begin{enumerate}[a.]
\item Prove that $V$ is an affine variety.
\item Determine $\I(V)$.
\end{enumerate}
This problem is quite a bit more challenging than the previous one—figuring out the proper analogue of equation (2) is not easy. Once we study the division algorithm in
Chapter 2, this exercise will become much easier.
\end{ejercicio}
\begin{solucion}
\begin{enumerate}[a.]
\item[]
\item Veamos que $V=\V(x^2-z,xz-y^2)$. Una inclusión es trivial, recíprocamente podemos suponer que $xyz\neq 0$, pues en otro caso se tendría $x=y=z=0$. Llamemos $t=y/x$. Entonces $t^2 = y^2/x^2 =xz/z = x$. Por tanto, $z=x^2=t^4$ e $y=tx=t^3$. Se tiene la igualdad.

\item Claramente $\gene{y^2-xz,z-x^2}\subseteq\I(V)$. Dado cualquier $f\in\R[x,y,z]$ podemos expresarlo como $f=h_1(y^2-xz)+h_2(z-x^2)+r$ con $h_1,h_2\in\R[x,y,z]$ y $r\in\R[x,y]$ pero con el exponente de $y$ a los sumo 1. Entonces, si $f\in\I(V)$ vamos a ver que $r=0$. Evaluando en los puntos de la forma $(t^2,t^3,t^4)$ nos queda $r(t^2,t^3)=0$ $\forall t \in \R$. Por tanto, $r=0$.

%\item Por el apartado anterior y por el Nullstellensatz $\I(V)=\sqrt{\gene{x^3-y^2, x^4-z^2, y^4-z^3}}$. Supongamos que $f\in \R[x,y,z]$ y $f(t^2,t^3,t^4)=0$ para todo $t\in\R$. Tenemos que $f(x,y,z)=\sum_{i,j,k}a_{i,j,k}x^iy^jz^k$. Entonces 
%\[
%f(t^2, t^3,t^4)=\sum_{i,j,k}a_{i,j,k}t^{2i}t^{3j}5t^{4k}=\sum_{i,j,k}a_{i,j,k}t^{2i+3j+4k}=0
%\]
%Entonces para cada entero $l\geq 0$ tenemos
%\[
%\underset{2i+3j+4k=l}{\sum_{i,j,k\geq 0}}a_{i,j,k}=0
%\]
%Esto fijo que no lleva a ninguna parte.
\end{enumerate}
\end{solucion}

\newpage
\begin{ejercicio}{1.4.13}
In Exercise 1.1.2, we showed that $x^2y+y^2x$ vanishes at all points of $\F_2^2$. More gener ally, let $I ⊆ \F_2[x, y]$ be the ideal of all polynomials that vanish at all points of $\F_2^2$. The goal of this exercise is to show that $I = \gene{x^2-x,y^2-y}$
\begin{enumerate}[a.]
\item Show that $\gene{x^2-x,y^2-y}\subset I$.
\item Show that every $f ∈ \F_2[x, y]$ can be written as $f = A(x^2 − x) + B(y^2 − y) + axy
+ bx + cy + d$, where $A, B ∈ \F_2[x, y]$ and $a, b, c, d ∈ \F_2$. Hint: Write f in the form $\sum_i p_i(x)y^i$ and use the division algorithm (Proposition 2 of §5) to divide each $p_i$ by $x^2 − x$. From this, you can write $f = A(x^2 − x) + q_1(y)x + q_2(y)$. Now divide $q_1$ and $q_2$ by $y^2 − y$. Again, this argument will become vastly simpler once we know the division algorithm from Chapter 2.
\item Show that $axy + bx + cy + d ∈ I$ if and only if $a = b = c = d = 0$.
\item Using parts (b) and (c), complete the proof that $I =\gene{x^2-x,y^2-y}$.
\item Express $x^2y + y^2x$ as a combination of $x^2-x$ and $y^2-y$.
\end{enumerate}
\begin{solucion}
\begin{enumerate}[a.]
\item[]
\item Es claro que si $f(x,y) = h_1(x^2-x)+h_2(y^2-y)$ entonces $f(0,0)=f(1,0)=f(0,1)=f(1,1)=0$. Por tanto $f\in I$, luego $\gene{x^2-x,y^2-y}\subset I$
\item Sabemos que podemos escribir $f=\sum_u p_i(x)y^i$. Utilizando el algoritmo de división, podemos dividir $p_i(x)$ por $x^2-x$ obteniendo $p_i(x) = m_i(x)(x^2-x)+r_i(x)$ con $\deg(r_i)\leq 1$ o $r_i=0$. Sumando, y utilizando que $r_i = a_ix+b_i$, obtenemos
$$
f(x,y) = \sum_i (m_i(x)(x^2-x) +r_i(x))y^i = A(x,y)(x^2-x) + q_1(y)x+q_2(y)
$$
Donde $A(x,y)=\sum_i m_i(x)y^i$, $q_1(y)=\sum_i a_iy^i$ y $q_2(y)=\sum_i b_i y^i$. Dividiendo $q_i$ entre $y^2-y$ obtenemos $q_i(y) = h_i(y)(y^2-y)+c_iy+d_i$, por lo que
$$
f(x,y)= A(x,y)(x^2-x) + B(x,y)(y^2-y) + c_1xy + d_1x+c_2y+d_2
$$
donde $B(x,y) = h_1(y)x+h_2(y)$.
\item Sea $f(x,y) = axy+bx+cy+d$. Si $f\in I$ entonces se anula en cada punto. Como $f(0,0)=d$, $d=0$. Dado que $f(1,0)=b$ y $f(0,1)=c$ entonces $b=c=0$. Finalmente, $f(1,1)=a$ por lo que $a=0$. El recíproco es trivial.
\item Sea $f\in I$ cualquiera, entonces podemos escriber $f$ según la fórmula obtenida en el apartado $(b)$, pero utilizando $(c)$, tenemos que puede escribirse simplemente como $A(x^2-x)+B(y^2-y)$. Pues si alguno de las otras constantes no fueran nulas, como $g = A(x^2-x)+B(y^2-y)\in \gene{x^2-x,y^2-y} \subset I$, tendríamos que $f-g\in I$, pero por la forma de $f-g$, por el apartado $(c)$, $f-g=0$. Por tanto, $f\in \gene{x^2-x,y^2-y}$.
\item $x^2y + y^2x=y(x^2-x)+x(y^2-y)$ (recordemos que el cuerpo es $\F_2$ y por tanto $1=-1$).
\end{enumerate}
\end{solucion} 
\end{ejercicio}
\newpage
\begin{ejercicio}{1.4.14}
This exercise is concerned with Proposition 8.
\begin{enumerate}[a.]
\item Prove that part (ii) of the proposition follows from part (i).
\item Prove the following corollary of the proposition: if V and W are affine varieties in $k^n$, then $V \not\subseteq W$ if and only if $\I(V)\not\supseteq\I(W)$.
\end{enumerate}
\end{ejercicio}
\begin{solucion}
\begin{enumerate}[a.]
\item[]
\item Es trivial, pues $V=W$ si y solo si $V\subset W$ y $W \subset V$. Ahora basta aplicar $(i)$.
\item Veamos una implicación por reducción al absurdo. Supongamos que $V\not \subset W$ pero $\I(W)\subset I(V)$. Entonces, por la Proposicion 8, $V\subset W$, lo cual es una contradicción con la hipótesis. El recíproco es análogo.
\end{enumerate}
\end{solucion}
\newpage
\begin{ejercicio}{1.4.15}
In the text, we defined $\I(V)$ for a variety $V ⊆ k^n$. We can generalize this as follows: if
$S ⊆ k^n$ is any subset, then we set
$$\I(S) = \{f ∈ k[x_1,\dots, x_n] \mid f (a_1,\dots, a_n) = 0\ \forall (a_1,\dots, a_n) ∈ S\}.$$
\begin{enumerate}[a.]
\item Prove that $\I(S)$ is an ideal.
\item Let $X = \{(a, a) ∈ \R^2 \mid a \neq 1\}$. By Exercise 8 of §2, we know that $X$ is not an affine
variety. Determine $\I(X)$. Hint: What you proved in Exercise 8 of §2 will be useful.
See also Exercise 10 of this section.
\item Let $\Z^n$ be the points of $\C^n$ with integer coordinates. Determine $\I(\Z^n)$. Hint: See Exercise
6 of §1.
\end{enumerate}
\begin{solucion}
\begin{enumerate}[a.]
\item[]
\item Análogo a cuando es una variedad.
\item $\I(X)=\I((t,t))=\langle x-y\rangle$.
\item $\I(\Z^n)=\I(\C^n)=\{0\}$. 
\end{enumerate}
\end{solucion}
\end{ejercicio}

\newpage

\begin{ejercicio}{1.4.16}
Here is more practice with ideals. Let $I$ be an ideal in $k[x_1,\dots , x_n]$.
\begin{enumerate}[a.]
\item[a.] Prove that $1 ∈ I$ if and only if $I = k[x_1,\dots , x_n]$.
\item[b.] More generally, prove that $I$ contains a nonzero constant if and only if $I = k[x_1,\dots, x_n]$.
\item[c.] Suppose $f , g ∈ k[x_1,\dots , x_n]$ satisfy $f^2, g^2 ∈ I$. Prove that $(f + g)^3 ∈ I$. Hint: Expand
$(f + g)^3$ using the Binomial Theorem.
\item[d.] Now suppose $f , g ∈ k[x_1,\dots , x_n]$ satisfy $f^r$ , $g^s ∈ I$. Prove that $(f + g)^{r+s−1} ∈ I$.
\end{enumerate}
\end{ejercicio}
\begin{solucion}
\begin{enumerate}[a.]
\item[]
\item Si $1\in I$, por ser ideal, $f\cdot 1\in I$ para todo $f\in k[x_1,\dots , x_n]$. Recíprocamente, si $I=k[x_1,\dotsc,x_n]$ es claro que $1\in I$.
\item Como $k$ es cuerpo, dada una constante $a$, podemos generar $1=aa^{-1}$, por lo que podemos aplicar el apartado anterior.
\item $(f+g)^3=f^3+3f^2g+3fg^2+g^3=ff^2+3f^2g+3fg^2+gg^2\in I$. 
\item Basta hacer lo mismo que hemos hecho antes con el desarrollo general. 
\end{enumerate}
\end{solucion}

\newpage

\begin{ejercicio}{1.4.17}
In the proof of Lemma 7, we showed that $x \not∈ 
\langle x^2, y^2\rangle$ in $k[x, y]$.
\begin{itemize}
\item[a.] Prove that $xy \not∈ 
\langle x^2, y^2\rangle$.
\item[b.] Prove that 1, $x$, $y$, $xy$ are the only monomials not contained in 
$\langle x^2, y^2\rangle$.
\end{itemize}
\end{ejercicio}
\begin{solucion}
\begin{itemize}
\item[]
\item[a.] Cualquier polinomio de $\langle x^2, y^2\rangle$ tendrá un término en $x^2$ o en $y^2$, cosa que $xy$ no tiene. 
\item[b.] Por el mismo razonamiento, esos monomios no están contenidos. Además, cualquier otro de $k[x,y]$ tiene algún término en $x^2$ o en $y^2$, luego está en el ideal. 
\end{itemize}
\end{solucion}

\newpage

\begin{ejercicio}{1.4.18}
In the text, we showed $\I(\{(0,0)\}) = \gene{x,y}$ in $k[x,y]$. 
\begin{enumerate}[a.]
\item Generalize this by proving that the origin $0\in k^n$ has the property that $\I(\{0\}) = \gene{x_1,\dotsc,x_n}$ in $k[x_1,\dotsc,x_n]$.
\item What does part (a) say about polynomials in $k[x_1,\dotsc,x_n]$ with zero constant term?
\end{enumerate}
\end{ejercicio}
\begin{solucion}
\begin{enumerate}[a.]
\item[]
\item Una contención es trivial, pues si $f= \sum g_i x_i$ entonces  $f(0)=0$, por lo que $f\in \I(\{0\})$. Como $I(S)$ es un ideal propio, basta probar que $\gene{x_1,\dotsc,x_n}$ es maximal, pero esto es claro pues $\gene{x_1,\dotsc,x_n} = k[x_1,\dotsc,x_n]\setminus k$. Luego si existiera otro ideal que lo contiene, este ha de tener necesariamente alguna unidad y por tanto sería el total.
\item Que siempre se anulan en el 0, o equivalentemente, que conforman el ideal $\gene{x_1,\dotsc,x_n}$.

\end{enumerate}
\end{solucion}
\newpage


\begin{ejercicio}{1.4.19}
One of the key ideas of this section is that a system of equations $f_1 =\cdots = f_s = 0$ gives the ideal $I = \gene{ f_1,\dotsc, f_s}$ of polynomial consequences. Now suppose that the system has a consequence of the form $f = g$ and we take the $m$-th power of each side to obtain $f^m = g^m$. In terms of the ideal $I$, this means that $f − g ∈ I$ should imply $f^m − g^m ∈ I$. Prove this by factoring $f^m − g^m$.
\end{ejercicio}
\begin{solucion}
Es trivial pues, si $f-g\in I$ entonces, dado que
$$
f^m-g^m = (f-g)\sum_{i=1}^{m-1}f^ig^{m-i}
$$
Luego $f^m-g^m \in I$.
\end{solucion}
\end{document}